Monads.v
@@ -1,0 +1,471 @@
+Require Import NPeano Arith Bool String List CpdtTactics.
+Set Implicit Arguments.
+
+(** A class definition defines an interface for some type.  In this
+   case, we say that types A that implement the Show interface have
+   a method named show that will convert them to a string. 
+
+   So we can use the generic method "show" on any type A that is
+   an instance of the Show class. 
+
+   In general, you can have multiple things in the interface that
+   depend upon the type A.
+*)
+Class Show(A:Type) := {
+  show : A -> string
+}.
+
+(** Here we define booleans as an instance of the Show class and
+   give a definition of the method.  *)
+Instance boolShow : Show bool := {
+  show := fun (b:bool) => (if b then "true" else "false") % string
+}.
+
+Compute show true.
+Compute show false.
+Eval compute in show 3.
+
+(** This doesn't work because we haven't said how to show a nat.
+ We get an even scarier message, 
+"[Error: vm_compute does not support existential variables.]"
+if we do [Compute show 3], because of that variable [?Show]. *)
+
+(** Now let's define nat as an instance of Show.  We first need
+   some helper functions to convert nats to strings. *)
+
+Definition digit2string(d:nat) : string := 
+  match d with 
+    | 0 => "0" | 1 => "1" | 2 => "2" | 3 => "3"
+    | 4 => "4" | 5 => "5" | 6 => "6" | 7 => "7"
+    | 8 => "8" | _ => "9"
+  end %string.
+
+(** Alas, it can be difficult to convince Coq that
+   this terminates.  So we give it fuel.  But, we
+   know how much fuel we should use in this case... *)
+Fixpoint digits'(fuel n:nat) (accum : string) : string := 
+  match fuel with 
+    | 0 => accum
+    | S fuel' => 
+      match n with 
+        | 0 => accum
+        | _ => let d := digit2string(n mod 10) in 
+               digits' fuel' (n / 10) (d ++ accum)
+      end
+  end.
+
+(** It's sufficient to use n as the fuel here since
+   we know we won't need to divide n by 10 more than
+   n times.  We could of course use log_10 n, but there's
+   no need to bother here. *)
+Definition digits (n:nat) : string := 
+  match digits' n n "" with 
+    | "" => "0"
+    | ds => ds
+  end %string.
+
+Require Import Recdef Nat Lia.
+Function digits''(n:nat) (accum:string) 
+            {measure (fun x:nat => x) n}: string :=
+  match n with
+  | 0 => accum
+  | _ => let d := digit2string(n mod 10) in
+         digits'' (n / 10) (d ++ accum)
+  end.
+Proof.
+  intros. apply Nat.div_lt ; lia.
+Defined.
+
+(* Now we can define our nat instance for the Show class. *)
+Instance natShow : Show nat := { 
+  show := digits
+}.
+
+Compute show 42.
+Compute show (10+2).
+
+(* Importantly, we still have the ability to show booleans. *)
+Compute show true.
+
+
+(** We can also parameterized instances, allowing us to show
+    data structures.
+
+    The following is a generic instance in that if we can have two types
+    A and B that are instances of the Show class, then we can
+    build a generic Show for the product type (A*B).
+*)
+Instance pairShow(A B:Type)(showA : Show A)(showB : Show B) : Show (A*B) := {
+  show := (fun p => "(" ++ (show (fst p)) ++ "," ++ (show (snd p)) ++ ")")
+            %string
+}.
+
+Compute show (3,4).
+Compute show (true,42).
+
+Print pairShow.
+
+(** Similarly, we can define a generic show for lists, as long
+   as the elements of the lists are show'able. *)
+Definition show_list{A:Type}{showA:Show A}(xs:list A) : string := 
+  ("[" ++ ((fix loop (xs:list A) : string := 
+             match xs with 
+               | nil => "]"
+               | h::nil => show h ++ "]"
+               | h::t => show h ++ "," ++ loop t
+             end) xs))%string.
+
+Instance listShow(A:Type)(showA:Show A) : Show (list A) := {
+  show := @show_list A showA
+}.
+
+Compute show (1::2::3::nil).
+Compute show (true::false::nil).
+Compute show ((1,true)::(42,false)::nil).
+Compute show ((1::2::3::nil)::(4::5::nil)::(6::nil)::nil).
+
+
+(** Here is another way to have an anonymous argument,
+    other than using the name [_]. *)
+Definition showOne {A:Type} `{Show A} (a:A) : string :=
+  "The value is " ++ show a.
+
+Compute showOne true.
+Compute showOne 7.
+
+Definition showTwo {A B:Type} {sa:Show A} `{Show B} (a:A) (b:B) : string :=
+  "First is " ++ show a ++ " and second is " ++ show b.
+
+Compute (showTwo true 7).
+
+(** Type classes are a powerful abstraction tool that fit very well
+    with some proof developments.
+
+    One tip is to make type classes as small and simple
+    as possible. For example, you probably want to separate out
+    the operations you want to use from the properties that
+    the implementation is expected to satisfy.
+*)
+
+
+(***********************************************************)
+
+(** Monads are very useful for modeling things that are not just
+   pure functions, that have some kind of external effect on the
+   world such as reading input or producing output. They're
+   essential for modeling statefulness a in pure, stateless,
+   functional language like Coq.
+
+   Now we define a generic class for Monads.  Here, it's not a type
+   that's a monad, but rather a type constructor (i.e., a function
+   from types to types, aka a functor.  Monads have two operations:
+   ret and bind.  
+
+   If we think of monads as a pattern for encoding effects, such
+   as exceptions or state or non-determinism, then we can think 
+   of "M A" as describing side-effecting computations that produce
+   a value of type A.  
+
+   The "ret" operation takes a pure (effect-free) value of type A
+   and injects it into the space of side-effecting computations.
+
+   The "bind" operation sequences two side-effecting computations,
+   allowing the latter to depend upon the value of the first one.
+*)
+
+Record Point (T:Type) : Type := {xCord:T; yCord:T}.
+
+Inductive Point' (T:Type) : Type :=
+| Build_Point':  T -> T -> Point' T
+.
+
+Check {| xCord := 2; yCord :=3 |}.
+
+Check (@Build_Point _ 2 3).
+
+Class Monad(M:Type -> Type) := 
+{
+  ret : forall {A:Type}, A -> M A ; 
+  bind : forall {A B:Type}, M A -> (A -> M B) -> M B
+}.
+
+(* As usual, we will use the more convenient notation for bind. *)
+Notation "x <- c1 ;; c2" := (bind c1 (fun x => c2)) 
+                             (right associativity, at level 84, c1 at next level).
+
+Notation "c1 ;; c2" := (bind c1 (fun _ => c2)) (at level 100, right associativity).
+
+Inductive IO :Type -> Prop := 
+| reti : forall A, A-> IO A
+| bindi : forall A B, IO A -> (A -> IO B) -> IO B
+| printString : string -> IO bool
+| readLine : IO string.
+
+
+(** One instance of the generic Monad class is the option monad
+   defined as follows. It's a bit like exceptions where there
+   is only one possible exception: None.
+ *)
+Instance OptionMonad : Monad option := 
+{
+  ret := fun {A:Type} (x:A) => Some x ; 
+  bind := fun {A B:Type} (x:option A) (f:A -> option B) =>
+            match x with 
+              | None => None
+              | Some y => f y
+            end
+}.
+
+(** How might we use this monad? We can 'fix' subtraction,
+    which ordinarily has odd semantics in Coq, so that any
+    computation of a negative number fails and that failure
+    propagates to the final result.
+*)
+
+Fixpoint subtract (x y:nat) : option nat := 
+  match x, y with 
+    | x, 0 => ret x
+    | 0, S _ => None
+    | S x', S y' => subtract x' y'
+  end.
+
+Inductive exp := 
+| Num : nat -> exp
+| Plus : exp -> exp -> exp
+| Minus : exp -> exp -> exp.
+
+Instance expShow : Show exp := {
+  show := fix show_exp (e:exp) : string := 
+              match e with 
+                | Num n => show n
+                | Plus e1 e2 => 
+                  "(" ++ (show_exp e1) ++ "+" ++ (show_exp e2) ++ ")"
+                | Minus e1 e2 => 
+                  "(" ++ (show_exp e1) ++ "-" ++ (show_exp e2) ++ ")"
+              end %string
+}.
+
+(** Now we can write an expression evaluator very conveniently: *)
+Fixpoint eval (e:exp) : option nat := 
+  match e with 
+    | Num n => ret n
+    | Plus e1 e2 => n1 <- eval e1 ;; 
+                    n2 <- eval e2 ;;
+                    ret (n1 + n2)
+    | Minus e1 e2 => n1 <- eval e1 ;; 
+                     n2 <- eval e2 ;;
+                     subtract n1 n2
+  end.
+
+Goal eval = fun x => None.
+unfold eval.
+simpl.
+Abort.
+
+Example e1 : exp := Plus(Num 2) (Minus(Num 0) (Num 1)).
+Compute (eval e1).
+(** That's better than normal evaluation: *)
+Compute 2 + (0 - 1).
+
+Print "+".
+
+Require Import String.
+Inductive Exn(A:Type) : Type := 
+| Result : A -> Exn A
+| Fail : string -> Exn A.
+Arguments Result {A}.
+Arguments Fail {A}.
+
+Instance ExnMonad : Monad Exn := 
+{
+  ret := fun {A:Type} (x:A) => Result x ; 
+  bind := fun {A B:Type} (x:Exn A) (f:A -> Exn B) =>
+            match x with 
+              | Result y => f y
+              | Fail s => Fail s
+            end
+}. 
+
+Fixpoint eval' (e:exp) : Exn nat := 
+  match e with 
+    | Num n => ret n
+    | Plus e1 e2 => n1 <- eval' e1 ;;
+                    n2 <- eval' e2 ;;
+                    ret (n1 + n2)
+    | Minus e1 e2 => n1 <- eval' e1 ;; 
+                     n2 <- eval' e2 ;;
+                     match subtract n1 n2 with 
+                       | None => Fail "underflow"
+                       | Some v => ret v
+                     end
+  end.
+
+Definition tryCatch {A} (e:Exn A) (s:string) (handler:Exn A) : Exn A := 
+  match e with 
+    | Fail s' => if string_dec s s' then handler else e
+    | _ => e
+  end.
+
+Definition eval_to_zero (e:exp) := 
+  tryCatch (eval' e) "underflow" (ret 0).
+
+Check eval_to_zero.
+Compute eval' (Minus (Num 2) (Num 5)).
+Compute eval_to_zero (Minus (Num 2) (Num 5)).
+
+
+(** We can also use monads to model state. *)
+
+Require Import List.
+Definition var := string.
+
+(** We define expressions equipped with an imperative
+    update: *)
+Inductive exp_s : Type := 
+| Var_s : var -> exp_s
+| Plus_s : exp_s -> exp_s -> exp_s
+| Times_s : exp_s -> exp_s -> exp_s
+| Set_s : var -> exp_s -> exp_s
+| Seq_s : exp_s -> exp_s -> exp_s
+| If0_s : exp_s -> exp_s -> exp_s -> exp_s.
+
+Definition state := var -> nat.
+Definition upd(x:var)(n:nat)(s:state) : state := 
+  fun v => if string_dec x v then n else s x.
+
+(** An evaluator can be written that passes the state
+    through everywhere, but it's tedious and error-prone: *)
+Fixpoint eval_s (e:exp_s)(s:state) : (state * nat) := 
+  match e with 
+    | Var_s x => (s, s x)
+    | Plus_s e1 e2 => 
+      let (s1, n1) := eval_s e1 s in
+      let (s2, n2) := eval_s e2 s1 in 
+      (s2, n1+n2)
+    | Times_s e1 e2 =>
+      let (s1, n1) := eval_s e1 s in
+      let (s2, n2) := eval_s e2 s1 in 
+      (s2, n1*n2)
+    | Set_s x e => 
+      let (s1, n1) := eval_s e s in 
+      (upd x n1 s1, n1)
+    | Seq_s e1 e2 => 
+      let (s1, n1) := eval_s e1 s in
+      eval_s e2 s1
+    | If0_s e1 e2 e3 => 
+      let (s1, n1) := eval_s e1 s in 
+      match n1 with 
+        | 0 => eval_s e2 s1
+        | _ => eval_s e3 s1
+      end
+  end.
+
+Definition state_comp(A:Type) : Type := state -> (state*A).
+
+Instance StateMonad : Monad state_comp := {
+  ret := fun {A:Type} (x:A) => (fun (s:state) => (s,x)) ; 
+  bind := fun {A B:Type} (c : state_comp A) (f: A -> state_comp B) => 
+            fun (s:state) => 
+              let (s',v) := c s in 
+              f v s'
+}.
+
+Definition read (x:var) : state_comp nat := 
+  fun s => (s, s x).
+
+Definition write (x:var) (n:nat) : state_comp nat := 
+  fun s => (upd x n s, n).
+
+
+(** The evaluator looks much cleaner with the state monad,
+    using the functions [read] and [write] to capture interaction
+    with the state.
+ *)
+Fixpoint eval_sm (e:exp_s) : state_comp nat := 
+  match e with 
+    | Var_s x => read x
+    | Plus_s e1 e2 => 
+      n1 <- eval_sm e1 ;;
+      n2 <- eval_sm e2 ;;
+      ret (n1 + n2)
+    | Times_s e1 e2 =>
+      n1 <- eval_sm e1 ;;
+      n2 <- eval_sm e2 ;;
+      ret (n1 * n2)
+    | Set_s x e => 
+      n <- eval_sm e ;;
+      write x n 
+    | Seq_s e1 e2 => 
+      _ <- eval_sm e1 ;; 
+      eval_sm e2
+    | If0_s e1 e2 e3 => 
+      n <- eval_sm e1 ;;
+      match n with 
+        | 0 => eval_sm e2
+        | _ => eval_sm e3 
+      end
+  end.
+
+(** We can also use monads to model nondeterministic
+    evaluation. *)
+
+Inductive exp_nd : Type := 
+| Choose_nd : list nat -> exp_nd
+| Plus_nd : exp_nd -> exp_nd -> exp_nd
+| Times_nd : exp_nd -> exp_nd -> exp_nd.
+
+Definition flatten {A:Type} (xs:list (list A)) := 
+  fold_right (fun x a => x ++ a) nil xs.
+
+Instance listMonad : Monad list := {
+  ret := fun {A:Type} (x:A) => (x::nil) ;
+  bind := fun {A B:Type} (c:list A) (f: A -> list B) => 
+            flatten (map f c)
+}.
+
+Fixpoint eval_nd (e:exp_nd) : list nat := 
+  match e with 
+    | Choose_nd ns => ns
+    | Plus_nd e1 e2 => 
+      n1 <- eval_nd e1 ;;
+      n2 <- eval_nd e2 ;;
+      ret (n1 + n2)
+    | Times_nd e1 e2 => 
+      n1 <- eval_nd e1 ;;
+      n2 <- eval_nd e2 ;;
+      ret (n1 * n2)
+  end.
+Import ListNotations.
+
+Goal eval_nd = fun _ => nil.
+unfold eval_nd. simpl.
+Abort.
+
+Compute eval_nd (Plus_nd (Choose_nd (1::2::nil)) (Choose_nd (3::4::nil))).
+
+(** Monads ideally satisfy the following laws, and a good exercise
+    is to try to show that any monad you define satisfies these laws. *)
+
+Class Monad_with_Laws (M: Type -> Type){MonadM : Monad M} :=
+{
+  m_left_id : forall {A B:Type} (x:A) (f:A -> M B), bind (ret x) f = f x ;
+  m_right_id : forall {A B:Type} (c:M A), bind c ret = c ;
+  m_assoc : forall {A B C} (c:M A) (f:A->M B) (g:B -> M C), 
+    bind (bind c f) g = bind c (fun x => bind (f x) g)
+}.
+
+(** This demonstration is easy for the option monad: *)
+
+Instance OptionMonadLaws : @Monad_with_Laws option _ := {}.
+  auto.
+  intros ; destruct c ; auto.
+  intros ; destruct c ; auto.
+Defined.
+
+(** In fact, not all monads we want to define will satisfy
+    these laws. In particular, the requirement of equality above
+    causes trouble when the monad contains functions, as in the
+    case of the state monad. We can get around that difficulty
+    by parameterizing the monad laws with an equivalence relation
+    that captures the notion of equality we want to use.
+*)
