lecture6_non_deterministic_imp.v
@@ -1,0 +1,505 @@
+Require Import Bool Arith String List CpdtTactics.
+Open Scope string_scope.
+
+Definition var := string.
+
+Inductive binop := Plus | Times | Minus.
+
+Inductive aexp : Type := 
+| Const : nat -> aexp
+| Var : var -> aexp
+| Binop : aexp -> binop -> aexp -> aexp.
+
+Inductive bexp : Type := 
+| Tt : bexp
+| Ff : bexp
+| Eq : aexp -> aexp -> bexp
+| Lt : aexp -> aexp -> bexp
+| And : bexp -> bexp -> bexp
+| Or : bexp -> bexp -> bexp
+| Not : bexp -> bexp.
+
+Inductive com : Type := 
+| Skip : com
+| Assign : var -> aexp -> com
+| Rand : var -> com
+| Seq : com -> com -> com
+| If : bexp -> com -> com -> com
+| While : bexp -> com -> com.
+
+Definition state := var -> nat.
+
+Definition get (x:var) (s:state) : nat := s x.
+
+Definition set (x:var) (n:nat) (s:state) : state := 
+  fun y => 
+    match string_dec x y with 
+        | left H => n 
+        | right H' => get y s
+    end.
+
+Definition eval_binop (b:binop) : nat -> nat -> nat := 
+  match b with 
+    | Plus => plus
+    | Times => mult
+    | Minus => minus
+  end.
+
+Fixpoint eval_aexp (e:aexp) (s:state) : nat := 
+  match e with 
+    | Const n => n
+    | Var x => get x s
+    | Binop e1 b e2 => (eval_binop b) (eval_aexp e1 s) (eval_aexp e2 s)
+  end.
+
+
+
+Fixpoint eval_bexp (b:bexp) (s:state) : bool := 
+  match b with 
+    | Tt => true
+    | Ff => false
+    | Eq e1 e2 => Nat.eqb (eval_aexp e1 s) (eval_aexp e2 s)
+    | Lt e1 e2 => Nat.ltb (eval_aexp e1 s) (eval_aexp e2 s)
+    | And b1 b2 => eval_bexp b1 s && eval_bexp b2 s
+    | Or b1 b2 => eval_bexp b1 s || eval_bexp b2 s
+    | Not b => negb (eval_bexp b s)
+  end.
+
+(** thisis a partial function. data structure*)
+Inductive eval_com : com -> state -> state -> Prop := 
+| Eval_skip : forall s, eval_com Skip s s
+| Eval_assign : forall s x e, eval_com (Assign x e) s (set x (eval_aexp e s) s)
+| Eval_rand: forall s x n, eval_com (Rand x) s (set x n s)
+| Eval_seq : forall c1 s0 s1 c2 s2, 
+               eval_com c1 s0 s1 -> eval_com c2 s1 s2 -> eval_com (Seq c1 c2) s0 s2
+| Eval_if_true : forall b c1 c2 s s',
+                   eval_bexp b s = true -> 
+                   eval_com c1 s s' -> eval_com (If b c1 c2) s s'
+| Eval_if_false : forall b c1 c2 s s',
+                   eval_bexp b s = false -> 
+                   eval_com c2 s s' -> eval_com (If b c1 c2) s s'
+| Eval_while_false : forall b c s, 
+                       eval_bexp b s = false -> 
+                       eval_com (While b c) s s
+| Eval_while_true : forall b c s1 s2 s3, 
+                      eval_bexp b s1 = true -> 
+                      eval_com c s1 s2 -> 
+                      eval_com (While b c) s2 s3 -> 
+                      eval_com (While b c) s1 s3.
+
+(** Notation "âŸ¨ A , S âŸ© â‡“ T" := (eval_com A S T) (at level 100). *)
+
+(* y := 1; x := 2; while 0 < x { y := y * 2; x := x - 1 } *)
+Definition prog1 := 
+  Seq (Assign "y" (Const 1))
+  (Seq (Assign "x" (Const 2))
+       (While (Lt (Const 0) (Var "x"))
+              (Seq (Assign "y" (Binop (Var "y") Times (Const 2)))
+                   (Assign "x" (Binop (Var "x") Minus (Const 1)))))).
+Ltac myinv H:= inversion H; subst; simpl in *; clear H.
+
+Theorem prog1_prop: forall s1 s2, eval_com prog1 s1 s2 -> get "x" s2 =0.
+Proof.
+unfold prog1; intros.
+Ltac foo :=
+match goal with
+| [H: eval_com (Seq _ _) _ _ |- _] => myinv H
+| [H: eval_com (Assign _ _) _ _ |- _] => myinv H
+end.
+
+Ltac bar :=
+match goal with
+| [H: eval_com (While _ _) _ _ |- _] => myinv H; try discriminate; repeat foo
+end.
+repeat foo.
+bar.
+bar. compute in H1. clear H1. myinv H7; simpl in *.
+- compute . reflexivity.
+- compute in H2. compute in H1. discriminate.
+Qed.
+
+
+Theorem seq_assoc : 
+  forall c1 c2 c3 s1 s2, 
+    eval_com (Seq (Seq c1 c2) c3) s1 s2 -> 
+    eval_com (Seq c1 (Seq c2 c3)) s1 s2.
+Proof.
+intros. repeat foo. apply Eval_seq with (s1:=s4).
+- assumption.
+- apply Eval_seq with (s1:=s3) ; assumption.
+
+(**
+Abhishek's proof
+intros. repeat foo. eauto using Eval_seq.
+*)
+Qed.
+
+
+
+Definition prog2 := While Tt Skip.
+
+Lemma wtce: forall c s1 s2, 
+    eval_com c s1 s2 -> c = prog2 -> False.
+Proof.
+ intros c s1 s2 H. unfold prog2.
+ induction H; repeat (intros; try discriminate).
+- myinv H0. discriminate.
+- myinv H2. apply IHeval_com2. reflexivity.
+Qed.
+
+Lemma while_true_cant_eval: forall s1 s2, ~ eval_com prog2 s1 s2.
+Proof.
+  unfold not, prog2. intros.
+  apply (wtce _ s1 s2 H eq_refl).
+Qed.
+
+
+Ltac myinj H := injection H ; intros ; subst ; clear H.
+
+Lemma while_true_imp_false : forall c s1 s2, eval_com c s1 s2 -> 
+                               forall b c', (forall s, eval_bexp b s = true) -> 
+                                             c = While b c' -> False. 
+Proof.
+  intros c s1 s2 H. induction H; repeat (intros; try discriminate).
+  - intros. myinv H1. congruence.
+  - intros. apply IHeval_com2 with (b0:=b0)(c':=c'); assumption.
+
+(** greg's proof
+  Ltac foo' := 
+  match goal with 
+    | [ H : ?x _ _ = ?x _ _ |- _ ] => myinj H
+    | [ H : forall s, eval_bexp _ s = _,
+        H' : eval_bexp _ ?s0 = _ |- _] => 
+      specialize (H s0) ; congruence
+    | [ H : forall b c, _ -> _ |- _ ] => eapply H ; eauto
+  end.
+
+  induction 1 ; intros ; try discriminate ; repeat foo'.
+*)
+Qed.
+  
+Lemma prog2_div : forall s1 s2, eval_com prog2 s1 s2 -> False.
+
+  Lemma prog2_div' : forall c s1 s2, eval_com c s1 s2 -> c = prog2 -> False.
+  Proof.
+    unfold prog2 ; induction 1; crush.
+  Qed.
+  Show.
+  intros. apply (prog2_div' _ _ _ H eq_refl).
+Qed.
+
+(** A simple chained tactic *)
+Ltac myinv' H := inversion H ; subst ; clear H ; simpl in *.
+
+(** This tactic applies when we have a hypothesis involving
+   eval_com of either a Seq or an Assign.  It inverts the
+   hypothesis, and performs substitution, simplifying things.
+*)
+Ltac eval_inv := 
+  match goal with 
+    | [ H : eval_com (Seq _ _) _ _ |- _ ] => myinv H
+    | [ H : eval_com (Assign _ _) _ _ |- _ ] => myinv H
+  end.
+
+(** This tactic inverts an eval_com of a While, producing
+   two sub-goals.  It tries to eliminate one (or both) of the goals
+   through discrimination on the hypotheses.
+*)
+Ltac eval_while_inv := 
+  match goal with
+    | [ H : eval_com (While _ _) _ _ |- _ ] => myinv H ; try discriminate
+  end.
+
+Theorem prog1_prop' : forall s1 s2, eval_com prog1 s1 s2 -> get "x" s2 = 0.
+Proof.
+  unfold prog1 ; intros.
+  repeat ((repeat eval_inv) ; eval_while_inv).
+  auto.
+Qed.
+
+Theorem seq_assoc' : 
+  forall c1 c2 c3 s1 s2, 
+    eval_com (Seq (Seq c1 c2) c3) s1 s2 -> 
+    eval_com (Seq c1 (Seq c2 c3)) s1 s2.
+  Lemma seq_assoc'' : 
+    forall c s1 s2, 
+      eval_com c s1 s2 -> 
+      forall c1 c2 c3,
+        c = Seq (Seq c1 c2) c3 -> 
+        eval_com (Seq c1 (Seq c2 c3)) s1 s2.
+  Proof.
+    (** Adds all of the eval_com constructors as hints for auto/crush *)
+    Hint Constructors eval_com.
+    induction 1 ; crush.
+    inversion H ; clear H ; subst ; 
+    econstructor ; eauto.
+  Qed.
+
+  intros. eapply seq_assoc'' ; eauto.
+Qed.
+
+(** Returns true when the variable x occurs as a subexpression of a *)
+Fixpoint contains (x:var) (a:aexp) : bool := 
+  match a with 
+    | Const _ => false
+    | Var y => if string_dec x y then true else false
+    | Binop a1 _ a2 => contains x a1 || contains x a2
+  end.
+
+SearchAbout (or).
+(** Changing a variable x that doesn't occur in a doesn't effect the 
+   value of a. *)
+Lemma eval_exp_set : 
+  forall s x n a,
+    contains x a = false -> 
+    eval_aexp a (set x n s) = eval_aexp a s.
+Proof.
+  induction a.
+  - intros. simpl. reflexivity.
+  - intros. simpl. myinv H. unfold set. unfold get. destruct (string_dec x v).
+   + discriminate.
+   + reflexivity.
+  - intros. myinv H. SearchAbout (_ || _ = false). 
+    apply orb_false_elim in H1. destruct H1. apply IHa1 in H. rewrite H.
+    apply IHa2 in H0. rewrite H0. reflexivity.
+
+(** Greg'g Proof
+destruct H1. eapply (or_introl ) in IHa1. destruct IHa1.
+    + Print or_intror . apply (or_intror (contains x a1 = contains x a1)).
+  induction a ; unfold set, get ; simpl ; unfold get ; crush.
+  destruct (string_dec x v) ; crush.
+  destruct (contains x a1) ; crush.
+*)
+Qed.
+
+(** 
+Problem Set 3
+In class we saw a relational small-step semantics for IMP. 
+Abhishek observed that the small-step semantics could be written
+as a function instead, since there is no recursion in the 'while' case.
+However, there is a loss of extensibility to some nondeterministic
+ features like concurrency.) Are these semantics really equivalent?
+Here is the relational semantics we saw in class:
+
+*)
+
+Inductive step_com : com -> state -> com -> state -> Prop := 
+| Step_assign: forall s x e,
+       step_com (Assign x e) s
+                (Skip) (set x (eval_aexp e s) s)
+| Step_rand: forall s x n, step_com (Rand x) s (Skip) (set x n s)
+| Step_seqL: forall c1 c2 c1' s s', step_com c1 s c1' s' ->
+                step_com (Seq c1 c2) s (Seq c1' c2) s'
+| Step_seqR: forall c s, step_com (Seq Skip c) s c s
+| Step_if_true: forall b c1 c2 s, eval_bexp b s = true ->
+                 step_com (If b c1 c2) s c1 s
+| Step_if_false: forall b c1 c2 s, eval_bexp b s = false ->
+                 step_com (If b c1 c2) s c2 s
+| Step_while: forall b c s,
+                 step_com (While b c) s
+                          (If b (Seq c (While b c)) Skip) s.
+
+SearchAbout (Some ).
+(** Problem1: Give a definition of the same small-step semantics,
+ as a function.
+*)
+
+(*Fixpoint  step_com_fn  (c: com) (s: state) : option (com * state) :=
+  match c with 
+    | Skip => None
+    | Assign v a => Some (Skip, (set v (eval_aexp a s) s))
+    | Seq c1 c2 => match (step_com_fn c1 s) with 
+                    | None => Some (c2, s) (** this is skip case*)
+                    | Some (c3, s1) => Some ((Seq c3 c2), s1)
+                   end
+    | If b c1 c2  => match eval_bexp b s with
+                        | true => Some (c1, s)
+                        | false => Some (c2, s)
+                       end
+    | While b c1 => Some ((If b (Seq c1 (While b c1)) Skip), s)
+   end.
+
+
+(** Prove that only Skip fails to step: *)
+Lemma progress : forall c s, step_com_fn c s = None -> c = Skip.
+Proof.
+  intro c.
+  induction c.
+(** ; intros; simpl in *; try( reflexivity); try (discriminate). *)
+  - intros. reflexivity. (**skip case*)
+  - intros. simpl in *. discriminate. (**Assign case*)
+  (**Seq case*)
+  - simpl in *. intros. destruct (step_com_fn c1 s) in H.
+    + destruct p. discriminate.
+    + discriminate.
+  - simpl in *. intros. destruct (eval_bexp b s) in H; discriminate.
+  - simpl in *. intros. remember ((eval_bexp b s)) as bb. 
+      destruct bb. 
+    + inversion H.
+    + discriminate.
+Qed.
+
+
+Lemma ss {A:Type} : forall (a b:A), Some a= Some b -> a =b.
+Proof using.
+  intros. inversion H. reflexivity.
+Qed.
+
+
+(** Prove that all steps in the functional semantics work in the
+   relational one.*) 
+Theorem forward_sim : forall c s c' s', 
+          step_com_fn c s = Some (c', s') -> step_com c s c' s'.
+Proof.
+ intro c. induction c.
+ * intros. simpl in *. discriminate.
+ * intros. simpl in *. myinv H. constructor.
+ * intros. simpl in *. remember (step_com_fn c1 s) as ss.
+   destruct ss.
+  + destruct p. myinv H. constructor. apply IHc1. 
+    symmetry in Heqss. assumption.
+  + inversion H. symmetry in Heqss. 
+    apply progress in Heqss. subst. constructor.
+ * intros. simpl in H. remember (eval_bexp b s) as bb.
+   destruct bb; myinv H; symmetry in Heqbb; constructor; apply Heqbb.
+ * intros. simpl in H. Print step_com. remember (eval_bexp b s) as bb.
+   destruct bb.
+   + myinv H. symmetry in Heqbb. constructor.
+   + myinv H. constructor.
+Qed.
+
+
+Theorem backward_sim : forall c s c' s', 
+  step_com c s c' s' -> step_com_fn c s = Some (c', s').
+Proof.
+intro c. induction c; intros; myinv H; try (reflexivity).
+* remember (step_com_fn c1 s) as stf. 
+    destruct stf.
+    - destruct p. apply IHc1 in H5. 
+      rewrite H5 in Heqstf. myinv Heqstf. reflexivity.
+    - symmetry in Heqstf. apply progress in Heqstf. 
+      subst. myinv H5.
+* rewrite H6; reflexivity.
+* rewrite H6; reflexivity.
+Qed.
+**)
+Require Import Coq.Logic.FunctionalExtensionality.
+
+(** We can commute assignments x:=ax; y:=ay  as long as the
+   variables don't overlap. *)
+Lemma assign_comm : 
+  forall x ax y ay s1 s2,
+    eval_com (Seq (Assign x ax) (Assign y ay)) s1 s2 -> 
+    contains x ay = false -> 
+    contains y ax = false -> 
+    x <> y -> 
+    forall s3, eval_com (Seq (Assign y ay) (Assign x ax)) s1 s3 -> s2 = s3.
+(*
+               forall z, get z s3 = get z s2.
+*)
+Proof.
+  intros.
+  repeat eval_inv.
+  repeat unfold set, get.
+  apply functional_extensionality. intro z.
+  destruct (string_dec x z); destruct (string_dec y z); try congruence.
+  (**
+    Greg's proof
+    specialize (eval_exp_set s1 y (eval_aexp ay s1) ax H1).
+    unfold set. crush.
+    specialize (eval_exp_set s1 x (eval_aexp ax s1) ay H0).
+    unfold set. crush.
+  *)
+  - subst. pose proof (eval_exp_set s1 y (eval_aexp ay s1) ax H1). 
+    rewrite <- H.
+    unfold set, get. reflexivity.
+  - subst. pose proof (eval_exp_set s1 x (eval_aexp ax s1) ay H0).
+    rewrite <- H. unfold set, get. reflexivity.
+Qed.
+
+
+Lemma assign_comm2 : 
+  forall x ax y ay s1 s2,
+    eval_com (Seq (Assign x ax) (Assign y ay)) s1 s2 -> 
+    contains x ay = false -> 
+    contains y ax = false -> 
+    x <> y -> 
+    eval_com (Seq (Assign y ay) (Assign x ax)) s1 s2.
+Proof.
+  intros.
+  remember (set x (eval_aexp ax (set y (eval_aexp ay s1) s1))
+                (set y (eval_aexp ay s1) s1)) as s3.
+  assert (eval_com (Seq (Assign y ay) (Assign x ax)) s1 s3).
+  rewrite Heqs3.
+  eauto.
+  specialize (assign_comm x ax y ay s1 s2 H H0 H1 H2 _ H3).
+  intro.
+  assert (s3 = s2).
+  Focus 2.
+  rewrite <- H5.
+  auto.
+  symmetry in H4. apply H4.
+  Qed.
+
+Inductive steps_com : com -> state -> com -> state -> Prop :=
+| Steps_none : forall c s, steps_com c s c s
+| Steps_some : forall c s c' s' c'' s'', step_com c s c' s' ->
+                steps_com c' s' c'' s'' -> steps_com c s c'' s''.
+
+Hint Constructors steps_com step_com eval_com.
+Lemma concat_seq : forall c1 c2 s1 s2 s3,
+              steps_com c1 s1 Skip s2 ->
+               steps_com c2 s2 Skip s3 ->
+                steps_com (Seq c1 c2) s1 Skip s3.
+Proof.
+intros c1 c2 s1 s2 s3.
+remember Skip as ss.
+intros p. induction p; subst; eauto.
+Qed.
+
+Theorem big_to_small:
+  forall c s s',
+   eval_com c s s' -> steps_com c s Skip s'.
+Proof.
+intros c s s1 H.
+induction H; eauto.
+* eapply concat_seq; eauto.
+* pose proof (concat_seq c (While b c) s1 s2 s3 IHeval_com1 IHeval_com2 ).
+  apply (Steps_some (While b c) s1 (If b (Seq c (While b c)) Skip) s1 Skip s3); eauto.
+  (** - auto. (** apply  Step_while.**)
+  - eauto. pose proof (Step_if_true b (Seq c (While b c)) Skip s1 H). eauto. **)
+Qed.
+
+Lemma steps_com_skip: forall s1 s2, steps_com Skip s1 Skip s2 -> s1 = s2.
+Proof.
+intros.
+myinv H.
+- reflexivity.
+- myinv H0.
+Qed.
+
+
+Theorem small_to_big:
+  forall c s s',
+   steps_com c s Skip s' -> eval_com c s s'.
+Proof.
+intros. remember Skip as ss. induction H;subst;auto.
+  specialize (IHsteps_com (@eq_refl _ Skip)).
+  revert dependent s''.
+  induction H.
+  - intros. inversion IHsteps_com; auto.
+  - intros. inversion IHsteps_com; auto.
+  - intros. rename s'' into f. myinv IHsteps_com. myinv H0. 
+    econstructor; [| apply H6].
+    apply IHstep_com; eauto.
+    apply  big_to_small. auto.
+  - intros.  
+    pose proof (Eval_skip s). econstructor.
+    + apply H.
+    + apply IHsteps_com.
+  - intros. auto.
+  - intros. auto.
+  - intros. myinv IHsteps_com; myinv H6; eauto.
+Qed.
+
+
